solve

HumanEvalLean/HumanEval127.lean
@@ -1,5 +1,114 @@
-def intersection : Unit :=
-  ()
+module
+
+import HumanEvalLean.Common.IsPrime
+
+/-!
+## Implementation
+-/
+
+def intersection (p : Int × Int) (q : Int × Int) : String :=
+  let l := max p.1 q.1
+  let r := min p.2 q.2
+  let length := r - l
+  if length > 0 ∧ isPrime length.toNat then "YES" else "NO"
+
+/-!
+## Tests
+-/
+
+example : intersection (1, 2) (2, 3) = "NO" := by native_decide
+example : intersection (-1, 1) (0, 4) = "NO" := by native_decide
+example : intersection (-3, -1) (-5, 5) = "YES" := by native_decide
+example : intersection (-2, 2) (-4, 0) = "YES" := by native_decide
+example : intersection (-11, 2) (-1, -1) = "NO" := by native_decide
+example : intersection (1, 2) (3, 5) = "NO" := by native_decide
+example : intersection (1, 2) (1, 2) = "NO" := by native_decide
+example : intersection (-2, -2) (-3, -2) = "NO" := by native_decide
+
+/-!
+## Verification
+-/
+
+theorem intersection_swap {p q} :
+    intersection p q = intersection q p := by
+  grind [intersection]
+
+theorem intersection_mem {p q} :
+    intersection p q ∈ ["YES", "NO"] := by
+  grind [intersection]
+
+theorem Int.mem_filter_mem_rco_toList_rco {l₁ r₁ l₂ r₂ : Int} {x : Int} :
+    x ∈ (l₁...r₁).toList.filter (· ∈ l₂...r₂) ↔ x ∈ ((max l₁ l₂)...(min r₁ r₂)) := by
+  grind [Std.Rco.mem_toList_iff_mem, Std.Rco.mem_iff]
+
+-- stolen from Init.Data.Range.Polymorphic.Lemmas, which is private
+private theorem eq_of_pairwise_lt_of_mem_iff_mem {lt : α → α → Prop} [asymm : Std.Asymm lt]
+    {l l' : List α} (hl : l.Pairwise lt) (hl' : l'.Pairwise lt)
+    (h : ∀ a, a ∈ l ↔ a ∈ l') : l = l' := by
+  induction l generalizing l'
+  · cases l'
+    · rfl
+    · rename_i x xs
+      specialize h x
+      simp at h
+  · rename_i x xs ih
+    cases l'
+    · specialize h x
+      simp at h
+    · have hx := (h x).mp (List.mem_cons_self)
+      cases List.mem_cons.mp hx
+      · rename_i y ys heq
+        cases heq
+        simp only [List.cons.injEq, true_and]
+        apply ih hl.tail hl'.tail
+        intro a
+        specialize h a
+        constructor
+        · intro haxs
+          replace h := h.mp (List.mem_cons_of_mem _ haxs)
+          cases List.mem_cons.mp h
+          · rename_i heq
+            cases heq
+            simp only [List.pairwise_cons] at hl
+            have := hl.1 x haxs
+            cases Std.Asymm.asymm _ _ this this
+          · simp [*]
+        · intro hays
+          replace h := h.mpr (List.mem_cons_of_mem _ hays)
+          cases List.mem_cons.mp h
+          · rename_i heq
+            cases heq
+            simp only [List.pairwise_cons] at hl'
+            have := hl'.1 x hays
+            cases Std.Asymm.asymm _ _ this this
+          · simp [*]
+      · rename_i y ys hx
+        simp only [List.pairwise_cons] at hl'
+        have hlt := hl'.1 _ hx
+        have hmem : y ∈ x :: xs := (h y).mpr List.mem_cons_self
+        cases List.mem_cons.mp hmem
+        · rename_i heq
+          cases heq
+          cases Std.Asymm.asymm _ _ hlt hlt
+        · simp only [List.pairwise_cons] at hl
+          have hgt := hl.1 y ‹_›
+          cases Std.Asymm.asymm _ _ hlt hgt
+
+-- not @[grind =] because `(· ∈ l₂...r₂)` cannot part of the discrimination key
+theorem Int.filter_mem_rco_toList_rco {l₁ r₁ l₂ r₂ : Int} :
+    (l₁...r₁).toList.filter (· ∈ l₂...r₂) = ((max l₁ l₂)...(min r₁ r₂)).toList := by
+  apply eq_of_pairwise_lt_of_mem_iff_mem (lt := LT.lt)
+  · apply List.Pairwise.filter
+    apply Std.Rco.pairwise_toList_lt
+  · apply Std.Rco.pairwise_toList_lt
+  · grind [mem_filter_mem_rco_toList_rco, Std.Rco.mem_toList_iff_mem]
+
+theorem intersection_spec {p q} :
+    intersection p q = "YES" ↔ IsPrime ((p.1...p.2).toList.filter (· ∈ q.1...q.2)).length := by
+  simp only [intersection, isPrime_eq_true_iff_isPrime, ite_eq_left_iff]
+  suffices h : (min p.2 q.2 - max p.1 q.1).toNat = ((p.1...p.2).toList.filter (· ∈ q.1...q.2)).length by
+    grind [isPrime_iff]
+  simp [Int.filter_mem_rco_toList_rco]
 
 /-!
 ## Prompt
@@ -12,7 +121,7 @@ def intersection(interval1, interval2):
     The given intervals are closed which means that the interval (start, end)
     includes both start and end.
     For each given interval, it is assumed that its start is less or equal its end.
-    Your task is to determine whether the length of intersection of these two 
+    Your task is to determine whether the length of intersection of these two
     intervals is a prime number.
     Example, the intersection of the intervals (1, 3), (2, 4) is (2, 3)
     which its length is 1, which not a prime number.
